<?xml version="1.0" encoding="windows-1252"?>
<rdf:RDF xmlns:rdf="http://www.w3.org/1999/02/22-rdf-syntax-ns#" xmlns:skos="http://www.w3.org/2004/02/skos/core#" xmlns:dc="http://purl.org/dc/elements/1.1/" xmlns:dcterms="http://purl.org/dc/terms/" xmlns:foaf="http://xmlns.com/foaf/0.1/">

<!-- This is a sample template only and is not the complete Platform Vocabulary. The template shows that the Platform Vocabulary contains two types of terms - Platform Types and Platform Instances. Platform Types are in the main BODC-sourced terms and Platform Instances are AODN-sourced terms. The template shows the skos encoding and relationships between the various terms -->		
	
<skos:ConceptScheme rdf:about="http://environment.data.gov.au/aodn/def/Platform">
  <dc:title>AODN/IMOS Platform Vocabulary</dc:title>
  <dc:description>This scheme defines the terms used in the AODN Platform Vocabulary. The AODN community has reused Platform Type terms from the BODC LO6 Platform Vocabulary. Some AODN Platform terms have narrower terms that are specific instances of Platform Types e.g. Aurora Australis is an instance of the Platform Type 'Ship'.</dc:description>
  <dc:creator>
   <foaf:Organization>
      <foaf:name>IMOS</foaf:name>
   </foaf:Organization>
  </dc:creator>
  <dc:publisher>
    <foaf:Person>
      <foaf:name>Natalia Atkins</foaf:name>
    </foaf:Person>
  </dc:publisher>
  <dc:rights>Freely Available For Reuse</dc:rights>
  <dcterms:issued>2014-05-29T14:25:38</dcterms:issued>
</skos:ConceptScheme>
	
<skos:Concept rdf:about="http://vocab.nerc.ac.uk/collection/L06/current/31/">	
  <skos:inScheme rdf:resource="http://environment.data.gov.au/aodn//def/Platform"/>
  <skos:prefLabel xml:lang="en">Research Vessel</skos:prefLabel>
  <skos:definition>A platform of any size operating on the surface of the water column in unpredictable locations that is specifically equipped manned and operated for scientific purposes, usually oceanographic research.</skos:definition>
  <dc:source>L06 SeaVox Platform Categories</dc:source>
  <dc:publisher>(BODC) NERC Vocabulary Server</dc:publisher>
  <skos:narrower rdf:resource="http://vocab.aodn.org.au/aodn/def/Platform/Instance/64"/>
  <skos:narrower rdf:resource="http://vocab.aodn.org.au/aodn/def/Platform/Instance/65"/>
  <skos:narrower rdf:resource="http://vocab.aodn.org.au/aodn/def/Platform/Instance/71"/>
</skos:Concept>

<skos:Concept rdf:about="http://vocab.aodn.org.au/aodn/def/Platform/Instance/64">	
  <skos:inScheme rdf:resource="http://environment.data.gov.au/aodn//def/Platform"/>
  <skos:prefLabel xml:lang="en">Southern Surveyor</skos:prefLabel>
  <skos:definition>CSIRO Marine National Facility research vessel. Built 1972 as Ranger Callisto (Norway), then became the UK registered (Kurd 1 Jan 1982), then renamed Kurdeen (2 Jan 1982). Renamed Southern Surveyor 31 Dec 1982 and registered in Australia from 15 Nov 1988. Length 66.16m. Active as at Mar 2012</skos:definition>
  <dc:source>AODN Platform Vocabulary</dc:source>
  <dc:publisher>IMOS</dc:publisher>
  <skos:broader rdf:resource="http://vocab.nerc.ac.uk/collection/L06/current/31/"/>
  <dc:description>callsign:VLHJ,commissioned:15-11-1988</dc:description>
  <dcterms:created> 2014-05-29T14:25:38 </dcterms:created>
  <dcterms:type>http://vocab.nerc.ac.uk/collection/L06/current/31/</dcterms:type>
</skos:Concept>
	
<skos:Concept rdf:about="http://vocab.aodn.org.au/aodn/def/Platform/Instance/65">	
  <skos:inScheme rdf:resource="http://environment.data.gov.au/aodn//def/Platform"/>
  <skos:prefLabel xml:lang="en">L'Astrolabe</skos:prefLabel>
  <skos:definition> Research vessel built 1986 as the Canadian vessel Fort Resolution, re-registered in France and renamed Austral Fish 12 May 1988, renamed L''Astrolabe 18 May 1989. Re-registered in French Southern Territories between 20 Jun 1995 - 11 Oct 2006, then re-registered in France. Owned by Bourbon Offshore Surf. Commissioned by TAAF and Institut Polaire Francais Paul-Emile Victor. Active as at Dec 2012.</skos:definition>
  <dc:source>AODN Platform Vocabulary</dc:source>
  <dc:publisher>IMOS</dc:publisher>
  <skos:broader rdf:resource="http://vocab.nerc.ac.uk/collection/L06/current/31/"/>
  <dc:description>callsign:FHZI,commissioned:18-05-1989</dc:description>
  <dcterms:created> 2014-05-29T14:25:38 </dcterms:created>
  <dcterms:type>http://vocab.nerc.ac.uk/collection/L06/current/31/</dcterms:type>
</skos:Concept>	
	
<skos:Concept rdf:about="http://vocab.aodn.org.au/aodn/def/Platform/Instance/71">	
  <skos:inScheme rdf:resource="http://environment.data.gov.au/aodn//def/Platform"/>
  <skos:prefLabel xml:lang="en">Aurora Australis</skos:prefLabel>
  <skos:definition> Research vessel owned by P and O Polar, length 94.91m.  Active as at Mar 2013.</skos:definition>
  <dc:source>AODN Platform Vocabulary</dc:source>
  <dc:publisher>IMOS</dc:publisher>
  <skos:broader rdf:resource="http://vocab.nerc.ac.uk/collection/L06/current/31/"/>
  <dc:description>callsign:VNAA,commissioned:1990</dc:description>
  <dcterms:created> 2014-05-29T14:25:38 </dcterms:created>
  <dcterms:type>http://vocab.nerc.ac.uk/collection/L06/current/31/</dcterms:type>
</skos:Concept>		
	
<skos:Concept rdf:about="http://vocab.nerc.ac.uk/collection/L06/current/32/">	
  <skos:inScheme rdf:resource="http://environment.data.gov.au/aodn//def/Platform"/>
  <skos:prefLabel xml:lang="en">Vessel Of Opportunity</skos:prefLabel>
  <skos:definition>A platform for purpose of commerce of any size operating on the surface of the water column in unpredictable locations that regularly collects scientific (oceanographic and meteorological) data (e.g. an instrumented cargo vessel).</skos:definition>
  <dc:source>L06 SeaVox Platform Categories</dc:source>
  <dc:publisher>(BODC) NERC Vocabulary Server</dc:publisher>
  <skos:narrower rdf:resource="http://vocab.aodn.org.au/aodn/def/Platform/Instance/101"/>
  <skos:narrower rdf:resource="http://vocab.aodn.org.au/aodn/def/Platform/Instance/102"/>
</skos:Concept>	
	
<skos:Concept rdf:about="http://vocab.aodn.org.au/aodn/def/Platform/Instance/101">	
  <skos:inScheme rdf:resource="http://environment.data.gov.au/aodn//def/Platform"/>
  <skos:prefLabel xml:lang="en">Stadacoma</skos:prefLabel>
  <skos:definition>General Cargo ship vessel, which is currently flying the flag of Bahamas (May 2013)</skos:definition>
  <dc:source>AODN Platform Vocabulary</dc:source>
  <dc:publisher>IMOS</dc:publisher>
  <skos:broader rdf:resource="http://vocab.nerc.ac.uk/collection/L06/current/32/"/>
  <dc:description>callsign:C6FS9,commissioned:1984</dc:description>
  <dcterms:created> 2014-05-29T14:25:38 </dcterms:created>
  <dcterms:type>http://vocab.nerc.ac.uk/collection/L06/current/32/</dcterms:type>
</skos:Concept>		
	
<skos:Concept rdf:about="http://vocab.aodn.org.au/aodn/def/Platform/Instance/102">	
  <skos:inScheme rdf:resource="http://environment.data.gov.au/aodn//def/Platform"/>
  <skos:prefLabel xml:lang="en">Wana Bhum</skos:prefLabel>
  <skos:definition>Container ship vessel, which is currently flying the flag of Thailand (May 2013)</skos:definition>
  <dc:source>AODN Platform Vocabulary</dc:source>
  <dc:publisher>IMOS</dc:publisher>
  <skos:broader rdf:resource="http://vocab.nerc.ac.uk/collection/L06/current/32/"/>
  <dc:description>callsign:HSB3403,commissioned:2005</dc:description>
  <dcterms:created> 2014-05-29T14:25:38 </dcterms:created>
  <dcterms:type>http://vocab.nerc.ac.uk/collection/L06/current/32/</dcterms:type>
	</skos:Concept>
	
</rdf:RDF>
